Added proofs for GroundSubstitution.from_atom_and_fact

ExistentialRules/ChaseSequence/Termination/Linear.lean
@@ -36,19 +36,70 @@ section SubstitutionsAndTriggers
 
   def extend_Substitutution  (s: GroundSubstitution sig) (v: sig.V) (c: GroundTerm sig) : GroundSubstitution sig := fun x => if x = v then c else s x
 
-  def matchVarorCons (s: GroundSubstitution sig) (t : VarOrConst sig) (gt : GroundTerm sig)(vars : List (sig.V)) : Option (GroundSubstitution sig) :=
+  def matchVarorConst (s: GroundSubstitution sig) (t : VarOrConst sig) (gt : GroundTerm sig)(vars : List (sig.V)) : Option (GroundSubstitution sig) :=
+  -- modifies Substitustion s such that t->gt if possible
     match t with
       | .const c => if gt = GroundTerm.const c then Option.some s else Option.none
       | .var v =>
-          if v ∈ vars -- Varas ist liste von variablen, die schon eine zuordnung in s haben
+          if v ∈ vars -- vars: List of variables, for which the substitutiion s is already 'properly' defined (has not just the dummy value anymore)
           then if gt = s v then Option.some s else Option.none--triit auf, wenn es für v schon eine andere substitution gab
           else some (extend_Substitutution s v gt)
 
+  theorem matchVarorConst.apply_var_or_const {t: VarOrConst sig} {gt: GroundTerm sig}: ∀ subs , matchVarorConst s t gt vars = some subs -> subs.apply_var_or_const t = gt := by
+    intro subs
+    unfold matchVarorConst
+    unfold GroundSubstitution.apply_var_or_const
+    cases t with
+    |var x =>
+      simp only
+      split
+      . simp only [Option.ite_none_right_eq_some, Option.some.injEq, and_imp]
+        intro eq_ap
+        intro eq_sub
+        rw[eq_ap]
+        simp only [eq_sub]
+      . unfold extend_Substitutution
+        simp only [Option.some.injEq]
+        intro fun_eq
+        rw[<-fun_eq]
+        simp
+    |const c =>
+      simp only
+      by_cases eq_c: gt=GroundTerm.const c
+      . simp[eq_c]
+      . simp[eq_c]
+
+
+  theorem matchVarorConst.noChange_vars {t: VarOrConst sig} : ∀ subs,  matchVarorConst s t gt vars = some subs -> v∈ vars ->  subs v = s v := by
+    intro subs
+    unfold matchVarorConst
+    cases t with
+    |var x =>
+      simp
+      by_cases var_x: x ∈ vars
+      . simp only [var_x, ↓reduceIte, Option.ite_none_right_eq_some, Option.some.injEq, and_imp]
+        intro a eq_sub var_v
+        simp[eq_sub]
+      . simp only [var_x, ↓reduceIte, Option.some.injEq]
+        unfold extend_Substitutution
+        intro a var_v
+        have v_ne_x:¬  v = x := by intro eq; rw[eq] at var_v; contradiction
+        rw[<- a]
+        simp only [ite_eq_right_iff]
+        intro v_eq_x
+        contradiction
+    |const c =>
+      simp only [Option.ite_none_right_eq_some, Option.some.injEq, and_imp];
+      intro a eq_sub var_v
+      simp[eq_sub]
+
+
   def matchTermList (s: GroundSubstitution sig) (vars : List (sig.V)) (l : List ((VarOrConst sig) × (GroundTerm sig))) : Option (GroundSubstitution sig) :=
+    --if possible, gives substitution subs s.t.  subs maps the List of VarOrConst to the List of GroundTerms
     match l with
     | .nil => Option.some s
     | (t, gt) :: ls =>
-      have s' := matchVarorCons s t gt vars
+      have s' := matchVarorConst s t gt vars
       match s' with
       |Option.none => Option.none
       |Option.some s' =>
@@ -56,21 +107,194 @@ section SubstitutionsAndTriggers
         | .var v => matchTermList s' (v::vars) ls
         | .const _ => matchTermList s' vars ls
 
+
+  theorem matchTermList.v_in_vars_noChange  {v: sig.V} :  ∀ s' s vars, v ∈ vars -> (matchTermList s vars ls) = some s' -> s' v = s v := by
+    intro s'
+    induction ls with
+    |nil =>
+      intro s vars mem_v
+      unfold matchTermList
+      simp only [Option.some.injEq]
+      intro s_eq_s'
+      rw[s_eq_s']
+    |cons f fs ih =>
+      unfold matchTermList
+      simp only
+      intro s vars var_v
+      cases h: matchVarorConst s f.fst f.snd vars with
+      |none => simp
+      |some s'' =>
+        have fun_eq: s'' v = s v := by
+          revert var_v;
+          apply matchVarorConst.noChange_vars;
+          rw[h];
+        simp only
+        cases f.fst with
+        |var x =>
+          simp only
+          intro a
+          rw[<- fun_eq]
+          have mem_v_ext : v ∈ (x::vars) := by simp[var_v]
+          apply ih
+          exact mem_v_ext
+          exact a
+        |const _ =>
+          simp only
+          rw[<-fun_eq]
+          revert var_v
+          apply ih
+
+--this is my current idea how to do this -> works keep it
+theorem matchTermList.apply_lists {l: List ((VarOrConst sig) × (GroundTerm sig))}:
+∀ subs s vars, matchTermList s vars l = some subs -> l.unzip.fst.map subs.apply_var_or_const = l.unzip.snd := by
+  intro subs
+  induction l with
+  |nil =>
+    simp
+  |cons f fs ih =>
+    intro s vars
+    unfold matchTermList
+    cases s': matchVarorConst s f.fst f.snd vars with
+    |none => simp
+    |some s'' =>
+      simp only[List.unzip_cons, List.map_cons, List.cons_eq_cons]
+      intro h
+      constructor
+      . have fun_eq_on_x: subs.apply_var_or_const f.fst = s''.apply_var_or_const f.fst := by
+          unfold GroundSubstitution.apply_var_or_const
+          revert h
+          cases f.fst with
+          |var x => simp only; apply matchTermList.v_in_vars_noChange; simp;
+          |const c => simp
+        rw[fun_eq_on_x]
+        apply matchVarorConst.apply_var_or_const
+        exact s'
+      . revert h
+        cases f.fst with
+        |var x => simp only; apply ih;
+        |const c => simp only; apply ih;
+
+    theorem matchTermList.some_if  {l: List ((VarOrConst sig) × (GroundTerm sig))}:
+      (∃ (subs: GroundSubstitution sig), l.unzip.fst.map subs.apply_var_or_const = l.unzip.snd ∧ (∀ (x:sig.V), x∈ vars -> s x = subs x) ) ->  ∃ subs, matchTermList s vars l = some subs  := by
+        intro h
+        apply Exists.elim h
+        intro a b
+        --unfold matchTermList
+        --have a := l.unzip.fst
+        induction l generalizing s vars with
+        |nil => unfold matchTermList; simp
+        |cons t ts ih =>
+          unfold matchTermList
+          simp only
+          unfold matchVarorConst
+          simp only[List.unzip_cons, List.map_cons, List.cons_eq_cons] at b
+          --unfold GroundSubstitution.apply_var_or_const at b
+          revert b
+          cases  t.fst with
+          |var v =>
+            simp only
+            intro b
+            by_cases v_mem_vars: v∈ vars
+            . simp only[v_mem_vars, b, ite_cond_eq_true];
+              have eq: a v = t.snd := by unfold GroundSubstitution.apply_var_or_const at b; simp only at b; exact b.left.left;
+              simp[eq]
+              apply ih
+              exists a
+              constructor
+              . exact b.left.right
+              . intro x x_in_v_vars; apply b.right; apply List.mem_of_mem_cons_of_mem; assumption;simp only[v_mem_vars]
+              constructor
+              . exact b.left.right
+              . intro x x_in_v_vars; apply b.right; apply List.mem_of_mem_cons_of_mem; assumption;simp only[v_mem_vars]
+
+            . simp[v_mem_vars]
+              have precond_s : (extend_Substitutution s v t.snd) v = t.snd := by unfold extend_Substitutution; simp
+              have x_vars_ext : ∀ x, x ∈ (v::vars) -> (extend_Substitutution s v t.snd) x = a x := by
+                intro x
+                simp[List.mem_cons, or_imp]
+                constructor
+                . intro xv; rw[xv] ; simp[precond_s]; apply Eq.symm; apply b.left.left;
+                . simp[extend_Substitutution];
+                  intro xv;
+                  by_cases h: x=v
+                  . rw[h] at xv; contradiction
+                  . simp[h]; revert xv;  apply b.right;
+              apply ih
+              exists a
+              constructor
+              . exact b.left.right
+              . assumption
+              constructor
+              . exact b.left.right
+              . assumption
+          |const c =>
+            simp only
+            intro b
+            rw[<-b.left.left]
+            unfold GroundSubstitution.apply_var_or_const
+            simp
+            apply ih
+            exists a
+            repeat exact And.intro b.left.right b.right
+
+
+
   -- The paper just calles this a homomorphism but we call this special kind of homomorphism a (ground) substitution.
   -- This will require auxiliary definitions.
   def GroundSubstitution.from_atom_and_fact (atom : FunctionFreeAtom sig) (fact : Fact sig) : Option (GroundSubstitution sig) :=
     if atom.predicate = fact.predicate
-    then matchTermList (fun _ => default) List.nil (List.zip atom.terms fact.terms)  --> wie kann ich die substiution initial definieren?
+    then matchTermList (fun _ => default) List.nil (List.zip atom.terms fact.terms)  -- calls matchTermList with a dummy substiution and the Notion, that no variables have a meaningful substitution yet (Empty List)
     else Option.none
 
 
   theorem GroundSubstitution.apply_function_free_atom_from_atom_and_fact {atom : FunctionFreeAtom sig} {fact : Fact sig} :
       ∀ subs, (GroundSubstitution.from_atom_and_fact atom fact) = some subs -> subs.apply_function_free_atom atom = fact := by
-    sorry
+        intro subs;
+        unfold from_atom_and_fact;
+        simp only [Option.ite_none_right_eq_some];
+        simp only [and_imp];
+        intro pred_eq;
+        simp only [apply_function_free_atom]
+        simp only [TermMapping.apply_generalized_atom]
+        intro s
+        have terms_length_eq : atom.terms.length = fact.terms.length := by simp only[GeneralizedAtom.arity_ok, pred_eq]
+        let l:= atom.terms.zip fact.terms
+        have a: l.unzip.fst = atom.terms:= by unfold l; apply List.unzip_zip_left; simp[terms_length_eq]
+        have b: l.unzip.snd = fact.terms := by unfold l; apply List.unzip_zip_right; simp[terms_length_eq]
+        have terms_eq : List.map subs.apply_var_or_const atom.terms = fact.terms
+          := by rw[<-a,<-b];apply matchTermList.apply_lists; assumption
+        simp[pred_eq, terms_eq]
+
+
 
   theorem GroundSubstitution.from_atom_and_fact_some_iff {atom : FunctionFreeAtom sig} {fact : Fact sig} :
-      ∃ subs, (GroundSubstitution.from_atom_and_fact atom fact) = some subs ↔ ∃ (subs : GroundSubstitution sig), subs.apply_function_free_atom atom = fact := by
-    sorry
+      (∃ subs, (GroundSubstitution.from_atom_and_fact atom fact) = some subs) ↔ ∃ (subs : GroundSubstitution sig), subs.apply_function_free_atom atom = fact := by
+        apply Iff.intro
+        . intro h;
+          apply Exists.elim h;
+          intro a b;
+          exists a;
+          apply GroundSubstitution.apply_function_free_atom_from_atom_and_fact
+          assumption
+        . intro h;
+          apply Exists.elim h
+          intro a b
+          unfold from_atom_and_fact
+          simp only [Option.ite_none_right_eq_some, exists_and_left]
+          constructor
+          . unfold apply_function_free_atom at b
+            unfold TermMapping.apply_generalized_atom at b
+            rw[<-b]
+          . apply matchTermList.some_if
+            simp only[List.not_mem_nil, false_implies, implies_true, and_true]
+            unfold apply_function_free_atom at b
+            unfold TermMapping.apply_generalized_atom at b
+            have len_eq: atom.terms.length = fact.terms.length := by rw[<-b]; simp;
+            simp only [len_eq, List.unzip_zip]
+            exists a
+            rw[<-b]
+
+
 
   def PreTrigger.from_rule_and_fact (rule : LinearRule sig) (fact : Fact sig) : Option (PreTrigger sig) :=
     (GroundSubstitution.from_atom_and_fact rule.body fact).map (fun subs => {
